- Did some rejigging of the tactics and added a new one called utp_prel_tac which handles typed relational conjectures - Added a sample program proof to the NFM 2014 paper

theories/poly/utp_poly_tac.thy
@@ -20,7 +20,7 @@ imports
   utp_poly_var
 begin
 
-text {* Theorem Attribute *}
+text {* Theorem Attributes *}
 
 ML {*
   structure evalp =
@@ -29,18 +29,45 @@ ML {*
 
 setup evalp.setup
 
-declare EvalP_simp [evalp]
-declare EvalP_TrueP [evalp]
-declare EvalP_FalseP [evalp]
-declare EvalP_NotP [evalp]
-declare EvalP_AndP [evalp]
-declare EvalP_OrP [evalp]
-declare EvalP_ImpliesP [evalp]
-declare EvalP_ClosureP [evalp]
-declare EvalP_RefP[evalp]
-declare EvalP_RenameP[evalp]
+ML {*
+  structure evalpp =
+    Named_Thms (val name = @{binding evalpp} val description = "evalpp theorems")
+*}
 
-declare Tautology_def [evalp]
+setup evalpp.setup
+
+ML {*
+  structure evalpr =
+    Named_Thms (val name = @{binding evalpr} val description = "evalpr theorems")
+*}
+
+setup evalpr.setup
+
+declare EvalP_simp [evalpp]
+declare EvalP_TrueP [evalpp]
+declare EvalP_FalseP [evalpp]
+declare EvalP_NotP [evalpp]
+declare EvalP_AndP [evalpp]
+declare EvalP_OrP [evalpp]
+declare EvalP_IffP [evalpp]
+declare EvalP_ImpliesP [evalpp]
+declare EvalP_ClosureP [evalpp]
+declare EvalP_RefP[evalpp]
+declare EvalP_RenameP[evalpp]
+
+declare Tautology_def [evalpp]
+declare less_eq_WF_PREDICATE_def [evalpp]
+declare CondR_def [evalpp, evalpr]
+
+declare EvalR_simp [evalpr]
+declare EvalR_refinement [evalpr]
+declare EvalR_TrueP_explicit [evalpr]
+declare EvalR_FalseP [evalpr]
+declare EvalR_NotP [evalpr]
+declare EvalR_OrP [evalpr]
+declare EvalR_AndP [evalpr]
+declare EvalR_SemiR [evalpr]
+declare EvalR_SkipR [evalpr]
 
 declare EmptyUS.rep_eq [evalp]
 declare InsertUS_rep_eq [evalp]
@@ -64,16 +91,30 @@ declare PrefixUL.rep_eq [evalp]
 declare PrefixeqUL.rep_eq [evalp]
 declare ULIST_transfer [evalp]
 
-
 ML {*
   fun utp_poly_simpset ctxt =
     (simpset_of ctxt)
       addsimps (evalp.get ctxt)
+      addsimps (evalpp.get ctxt)
       addsimps (closure.get ctxt)
       addsimps (typing.get ctxt)
       addsimps (defined.get ctxt)
       addsimps (unrest.get ctxt);
 *}
+
+ML {*
+  fun utp_prel_simpset ctxt =
+    (simpset_of ctxt)
+      addsimps (evalp.get ctxt)
+      addsimps (evalpr.get ctxt)
+      addsimps (closure.get ctxt)
+      addsimps (typing.get ctxt)
+      addsimps (defined.get ctxt)
+      addsimps (urename.get ctxt)
+      addsimps (unrest.get ctxt);
+*}
+
+declare binding_equiv_trans [intro]
 
 ML {*
   fun utp_poly_tac thms ctxt i =
@@ -83,9 +124,20 @@ ML {*
 
 ML {*
   fun utp_poly_auto_tac thms ctxt i =
-    CHANGED ((
-      (asm_full_simp_tac (utp_poly_simpset ctxt)) THEN_ALL_NEW
-      (SELECT_GOAL (auto_tac ctxt))) i)
+    CHANGED (
+      (SELECT_GOAL (auto_tac (map_simpset (fn _ => (utp_poly_simpset ctxt)) ctxt)) i))
+*}
+
+ML {*
+  fun utp_prel_tac thms ctxt i =
+    CHANGED (
+      TRY (asm_full_simp_tac (utp_prel_simpset ctxt) i))
+*}
+
+ML {*
+  fun utp_prel_auto_tac thms ctxt i =
+    CHANGED (
+      (SELECT_GOAL (auto_tac (map_simpset (fn _ => (utp_prel_simpset ctxt) addsimps (@{thms "relcomp_unfold"})) ctxt)) i))
 *}
 
 method_setup utp_poly_tac = {*
@@ -99,6 +151,18 @@ method_setup utp_poly_auto_tac = {*
   (fn thms => fn ctxt =>
     SIMPLE_METHOD' (utp_poly_auto_tac thms ctxt))
 *} "proof tactic for polymorphic predicates with auto"
+
+method_setup utp_prel_tac = {*
+  Attrib.thms >>
+  (fn thms => fn ctxt =>
+    SIMPLE_METHOD' (utp_prel_tac thms ctxt))
+*} "proof tactic for polymorphic relations"
+
+method_setup utp_prel_auto_tac = {*
+  Attrib.thms >>
+  (fn thms => fn ctxt =>
+    SIMPLE_METHOD' (utp_prel_auto_tac thms ctxt))
+*} "proof tactic for polymorphic relations with auto"
 
 end
 
